First commit of an accepted correctness proof!

ParseTree.v
@@ -1,5 +1,5 @@
 Require Import Grammar.
-
+Require Import String.
 (* Type variable seems to be cluttering up the definitions below. *)
 Inductive parse_tree {A} :=
 | Leaf : A -> parse_tree
@@ -19,3 +19,50 @@ Definition isNode {A} (tree : (@parse_tree A)) : bool :=
 
 Definition isLeaf {A} (tree : (@parse_tree A)) : bool :=
   negb (isNode tree).
+
+(* New stuff is here *)
+
+Inductive tree :=
+| Lf : string -> tree
+| Nd : string -> forest -> tree
+with forest :=
+     | Fnil : forest
+     | Fcons : tree -> forest -> forest.
+
+Fixpoint appForest xs ys :=
+  match xs with
+  | Fnil => ys
+  | Fcons t xs' => Fcons t (appForest xs' ys)
+  end.
+  
+
+Fixpoint revForest ts :=
+  match ts with
+  | Fnil => Fnil
+  | Fcons t ts' => appForest (revForest ts') (Fcons t Fnil)
+  end.
+
+Scheme tree_ind' := Induction for tree Sort Prop
+  with forest_ind' := Induction for forest Sort Prop.
+
+Require Import List.
+Import ListNotations.
+
+Inductive derTree {g : grammar} : symbol -> list string -> tree -> Prop :=
+| derT : forall (y : string),
+    derTree (T y) [y] (Lf y)
+| derNT : forall (x : string) (gamma : list symbol) (tokens : list string) (subtrees : forest),
+    In (NT x, gamma) g ->
+    derForest gamma tokens subtrees ->
+    derTree (NT x) tokens (Nd x subtrees)
+with derForest {g : grammar} : list symbol -> list string -> forest -> Prop :=
+     | derFnil : derForest [] [] Fnil
+     | derFcons : forall (hdRoot : symbol)
+                         (prefix : list string)
+                         (hdSubtree : tree)
+                         (tlRoots : list symbol)
+                         (suffix : list string)
+                         (tlSubtrees : forest),
+         derTree hdRoot prefix hdSubtree ->
+         derForest tlRoots suffix tlSubtrees ->
+         derForest (hdRoot :: tlRoots) (prefix ++ suffix) (Fcons hdSubtree tlSubtrees).
