ParserCorrectnessProofs.v
@@ -116,27 +116,37 @@ Proof.
     + exfalso. apply n. subst. reflexivity.
 Defined.
 
+Print tree_ind'.
+
+Definition isNd tr :=
+  match tr with
+  | Lf _ => false
+  | Nd _ _ => true
+  end.
+
 Lemma nt_derives_node :
   forall tbl x input fuel tree suffix,
     mkTree tbl (NT x) input fuel = (Some tree, suffix) ->
-    isNode tree = true.
+    isNd tree = true.
 Proof.
   intros. destruct fuel.
   - simpl in H. inv H.
   - simpl in H. destruct input.
     + inv H.
     + destruct (parseTableLookup (NT x) (T s) tbl).
-      * destruct (mkSubtrees tbl l (s :: input) [] fuel) in H.
+      * destruct (mkForest tbl l (s :: input) fuel) in H.
         destruct o.
         { inv H. simpl. reflexivity. }
         inv H.
       * inv H.
 Defined.
 
+Definition isLf tr := negb (isNd tr).
+
 Lemma t_derives_Leaf :
   forall tbl y input fuel tree suffix,
     mkTree tbl (T y) input fuel = (Some tree, suffix) ->
-    isLeaf tree = true.
+    isLf tree = true.
 Proof.
   intros. destruct fuel.
   - inv H.
@@ -147,35 +157,110 @@ Proof.
       * inv H.
 Defined.
 
-Lemma mkSubtreesCorrect :
-  forall (g     : grammar)
-         (tbl   : parse_table)
-         (gamma : list symbol)
-         (input : list string)
-         (fuel  : nat)
-         (acc   : list (@parse_tree string))
-         (subtrees  : list parse_tree)
-         (suffix : list string),
-    isParseTableFor tbl g -> 
-    mkSubtrees tbl gamma input acc fuel =
-    (Some subtrees, suffix) ->
-    exists prefix,
-      (prefix ++ suffix)%list = input /\
-      (@derivesList g) gamma prefix subtrees.
-Proof. Abort.  
+(* Get rid of this and infer membership from isParseTableFor *)
+Lemma silly_In_Grammar : forall (g :grammar) x gamma,
+    In (NT x, gamma) g.
+Proof. Admitted.
 
-Lemma parserCorrect :
-  forall (g     : grammar)
-         (tbl   : parse_table)
-         (start : symbol)
-         (input : list string)
-         (fuel  : nat)
-         (tree  : parse_tree)
-         (suffix : list string),
-    isParseTableFor tbl g -> 
-    mkTree tbl start input fuel = (Some tree, suffix) ->
+
+Theorem parse_correct : forall tbl g sym input tr suffix fuel,
+    isParseTableFor tbl g ->
+    mkTree tbl sym input fuel = (Some tr, suffix) ->
     exists prefix,
       (prefix ++ suffix)%list = input /\
-      (@derives g) start prefix tree.
+      (@derTree g) sym prefix tr.
 Proof.
-Admitted.
+  intros.
+  generalize dependent sym.
+  generalize dependent input.
+  generalize dependent suffix.
+  generalize dependent fuel. 
+  induction tr using tree_ind' with
+      (P := fun tr =>
+              forall fuel suffix input sym,
+                mkTree tbl sym input fuel = (Some tr, suffix) ->
+                exists prefix,
+                  (prefix ++ suffix)%list = input /\
+                  (@derTree g) sym prefix tr)
+      (P0 := fun subtrees =>
+               forall fuel suffix input gamma,
+                 mkForest tbl gamma input fuel = (Some subtrees, suffix) ->
+                 exists prefix,
+                   (prefix ++ suffix)%list = input /\
+                   (@derForest g) gamma prefix subtrees).
+  - intros. destruct fuel.
+    + inv H0.
+    + destruct sym.
+      * destruct input.
+        { inv H0. }
+        simpl in H0.
+        destruct (cmpSymbol (T s0) (T s1)) eqn:Hcmp.
+        { inv H0. exists [s1]. split.
+          { reflexivity. }
+          apply eq_sym_eq_T in Hcmp. subst.
+          apply derT. }
+        inv H0.
+      * apply nt_derives_node in H0. inv H0.
+  - intros. destruct fuel.
+    + inv H0.
+    + destruct sym.
+      * apply t_derives_Leaf in H0. inv H0.
+      * destruct input.
+        { inv H0. }
+        simpl in H0.
+        destruct (parseTableLookup (NT s0) (T s1) tbl) eqn:Htbl.
+        { destruct (mkForest tbl l (s1 :: input) fuel)
+                   eqn:Hforest.
+          { destruct o.
+            { inv H0.
+              apply IHtr in Hforest.
+              destruct Hforest.
+              exists x. destruct H0. split.
+              { assumption. }
+              inv H1.
+              { apply derNT with (gamma := nil).
+                { apply silly_In_Grammar. }
+                apply derFnil. }
+              apply derNT with (gamma := (hdRoot :: tlRoots)).
+              { apply silly_In_Grammar. }
+              apply derFcons.
+              { assumption. }
+              assumption. }
+            inv H0. }}
+        inv H0.
+  - intros. simpl in H0. destruct fuel.
+    + inv H0.
+    + destruct gamma.
+      * simpl in H0. inv H0.
+        exists nil. split.
+        { reflexivity. }
+        apply derFnil.
+      * exfalso.
+        simpl in H0.
+        destruct (mkTree tbl s input fuel).
+        destruct o.
+        { destruct (mkForest tbl gamma l fuel).
+          destruct o.
+          { inv H0. }
+          inv H0. }
+        inv H0.
+  - intros. destruct fuel.
+    + inv H0.
+    + destruct gamma.
+      * inv H0.
+      * simpl in H0. destruct (mkTree tbl s input fuel) eqn:Htree.
+        destruct o.
+        { destruct (mkForest tbl gamma l fuel) eqn:Hforest.
+          destruct o.
+          { inv H0.
+            apply IHtr in Htree. destruct Htree. destruct H0.
+            apply IHtr0 in Hforest. destruct Hforest.
+            destruct H2. subst.
+            exists (x ++ x0)%list. split.
+            { rewrite app_assoc. reflexivity. }
+            apply derFcons.
+            { assumption. }
+            assumption. }
+          inv H0. }
+        inv H0.
+Defined.
