ParserTests.v
@@ -28,6 +28,30 @@ Definition parseTree1 :=
               Node "E"
                    [Leaf "num"; Leaf "=="; Leaf "num"]]].
 
+Definition E_tree :=
+  Nd "E"
+     (Fcons (Lf "num")
+            (Fcons (Lf "==")
+                   (Fcons (Lf "num")
+                          Fnil))).
+
+Definition S_print_tree :=
+  Nd "S"
+     (Fcons (Lf "print")
+            (Fcons E_tree Fnil)).
+
+Definition parseTree2 :=
+  Nd "S"
+     (Fcons (Lf "if")
+            (Fcons E_tree
+                   (Fcons (Lf "then")
+                           (Fcons S_print_tree
+                                  (Fcons (Lf "else")
+                                         (Fcons S_print_tree
+                                                Fnil)))))).
+
+
+
 Example test1 :
   parse g311ParseTable "S" input1 100 = Accept parseTree1.
 Proof. cbv. reflexivity. Defined.
@@ -35,5 +59,7 @@ Proof. cbv. reflexivity. Defined.
 (* The new definition works, too! *)
 Example test2 :
   mkTree g311ParseTable (NT "S") input1 100 =
-  (Some parseTree1, nil).
+  (Some parseTree2, nil).
 Proof. simpl. reflexivity. Defined.
+
+Compute (mkTree g311ParseTable (NT "S") input1 100).
